<?xml version="1.0" encoding="utf-8"?>
<rdf:RDF
	xmlns:owl="http://www.w3.org/2002/07/owl#"
	xmlns:prov="http://www.w3.org/ns/prov#"
	xmlns:rdfs="http://www.w3.org/2000/01/rdf-schema#"
	xmlns:dc="http://purl.org/dc/elements/1.1/"
	xmlns:oa="http://www.w3.org/ns/oa#"
	xmlns:rdf="http://www.w3.org/1999/02/22-rdf-syntax-ns#"
	xmlns:dcterms="http://purl.org/dc/terms/"
	xmlns:foaf="http://xmlns.com/foaf/0.1/"
	xmlns:crowds="http://www.digirati.com/ns/crowds#"
	xmlns:xsd="http://www.w3.org/2001/XMLSchema#"
    >
	<rdf:Property rdf:about="http://www.digirati.com/ns/crowds#uiInputType">
		<rdfs:isDefinedBy rdf:resource="http://www.digirati.com/ns/crowds#"/>
		<rdfs:comment>Defines which user input control is rendered in a crowd-sourcing system, for capturing the value of an annotation. For example: textbox, listbox, dropdown. Options are defined by the Madoc vocabulary.</rdfs:comment>
		<rdfs:label>uiInputType</rdfs:label>
	</rdf:Property>
	<rdf:Property rdf:about="http://www.digirati.com/ns/crowds#uiInputDefaultValue">
		<rdfs:isDefinedBy rdf:resource="http://www.digirati.com/ns/crowds#"/>
		<rdfs:comment>Provides default value for any input control.</rdfs:comment>
		<rdfs:label>uiInputDefaultValue</rdfs:label>
	</rdf:Property>
	<rdf:Property rdf:about="http://www.digirati.com/ns/crowds#uiInputOptions">
		<rdfs:isDefinedBy rdf:resource="http://www.digirati.com/ns/crowds#"/>
		<rdfs:comment>Provides options refining the rendering of an input control, such as values for a drop-down. </rdfs:comment>
		<rdfs:label>uiInputOptions</rdfs:label>
	</rdf:Property>
	<rdf:Property rdf:about="http://www.digirati.com/ns/crowds#uiSelectorType">
		<rdfs:isDefinedBy rdf:resource="http://www.digirati.com/ns/crowds#"/>
		<rdfs:comment>Defines which user input control is rendered in a crowd-sourcing system, for selecting the target of an annotation.</rdfs:comment>
		<rdfs:label>uiSelectorType</rdfs:label>
	</rdf:Property>
	<rdf:Property rdf:about="http://www.digirati.com/ns/crowds#uiSelectorValue">
		<rdfs:isDefinedBy rdf:resource="http://www.digirati.com/ns/crowds#"/>
		<rdfs:comment>Defines which value is preset for a user input control as rendered in a crowd-sourcing system, e.g. preset XYWH coordinates for a box, or preset XY coordinates for a pointer.</rdfs:comment>
		<rdfs:label>uiSelectorValue</rdfs:label>
	</rdf:Property>
	<rdf:Property rdf:about="http://www.digirati.com/ns/crowds#uiComponent">
		<rdfs:isDefinedBy rdf:resource="http://www.digirati.com/ns/crowds#"/>
		<rdfs:comment>Provides a hint for which annotation studio component should load the annotation: resource provider; transcription; bookmarking; flagging; tagging, etc.</rdfs:comment>
		<rdfs:label>uiComponent</rdfs:label>
	</rdf:Property>
	<rdf:Property rdf:about="http://www.digirati.com/ns/crowds#externalResourceModel">
		<rdfs:isDefinedBy rdf:resource="http://www.digirati.com/ns/crowds#"/>
		<rdfs:comment>Dereference to return a description, model, or schema for the creation of an external resource from captured content.</rdfs:comment>
		<rdfs:label>externalResourceModel</rdfs:label>
	</rdf:Property>
	<rdf:Property rdf:about="http://www.digirati.com/ns/crowds#uiGroup">
		<rdfs:isDefinedBy rdf:resource="http://www.digirati.com/ns/crowds#"/>
		<rdfs:comment>Defines how a group of UI input elements should be rendered as a group.</rdfs:comment>
		<rdfs:label>uiGroup</rdfs:label>
	</rdf:Property>
	<rdf:Property rdf:about="http://www.digirati.com/ns/crowds#uiFormGroup">
		<rdfs:isDefinedBy rdf:resource="http://www.digirati.com/ns/crowds#"/>
		<rdfs:comment>Defines a named form group of UI input elements which should be rendered as a group (if uiGroup is set to form).</rdfs:comment>
		<rdfs:label>uiFormGroup</rdfs:label>
	</rdf:Property>
	<rdf:Property rdf:about="http://www.digirati.com/ns/crowds#uiMultiple">
		<rdfs:isDefinedBy rdf:resource="http://www.digirati.com/ns/crowds#"/>
		<rdfs:range rdf:resource="xsd:boolean"/>
		<rdfs:comment>Boolean: defines whether a particular UI group or element can be used multiple times, for example, if tagging an image with two different people.</rdfs:comment>
		<rdfs:label>uiMultiple</rdfs:label>
	</rdf:Property>
	<rdf:Property rdf:about="http://www.digirati.com/ns/crowds#uiRequired">
		<rdfs:isDefinedBy rdf:resource="http://www.digirati.com/ns/crowds#"/>
		<rdfs:range rdf:resource="xsd:boolean"/>
		<rdfs:comment>Boolean: defines whether a particular UI group or element MUST have a value.</rdfs:comment>
		<rdfs:label>uiRequired</rdfs:label>
	</rdf:Property>
	<rdf:Property rdf:about="http://www.digirati.com/ns/crowds#uiHidden">
		<rdfs:isDefinedBy rdf:resource="http://www.digirati.com/ns/crowds#"/>
		<rdfs:range rdf:resource="xsd:boolean"/>
		<rdfs:comment>Boolean: defines whether a particular UI group or element is displayed in the UI.</rdfs:comment>
		<rdfs:label>uiHidden</rdfs:label>
	</rdf:Property>
	<rdf:Property rdf:about="http://www.digirati.com/ns/crowds#uiChoice">
		<rdfs:isDefinedBy rdf:resource="http://www.digirati.com/ns/crowds#"/>
		<!--<rdfs:range rdf:resource="xsd:boolean"/>-->
		<rdfs:comment>Boolean: defines whether a particular UI group is a choice, i.e. do not render all of these together, provide a choice between them.</rdfs:comment>
		<rdfs:label>uiChoice</rdfs:label>
	</rdf:Property>
	<rdf:Property rdf:about="http://www.digirati.com/ns/crowds#derivedAnnoCombine">
		<rdfs:isDefinedBy rdf:resource="http://www.digirati.com/ns/crowds#"/>
		<rdfs:range rdf:resource="xsd:boolean"/>
		<rdfs:comment>Boolean: defines whether a particular set of putative annotations are to be combined into multiple annotation bodies in the same annotation (True), or stored as separate annotations (False).</rdfs:comment>
		<rdfs:label>derivedAnnoCombine</rdfs:label>
	</rdf:Property>
	<rdf:Property rdf:about="http://www.digirati.com/ns/crowds#derivedAnnoSerialize">
		<rdfs:isDefinedBy rdf:resource="http://www.digirati.com/ns/crowds#"/>
		<rdfs:range rdf:resource="xsd:boolean"/>
		<rdfs:comment>Boolean: defines whether an annotation body or set of annotation bodies should be stored as a serialized TextualBody, i.e. as a string.</rdfs:comment>
		<rdfs:label>derivedAnnoSerialize</rdfs:label>
	</rdf:Property>
	<rdf:Property rdf:about="http://www.digirati.com/ns/crowds#derivedAnnoExternalize">
		<rdfs:isDefinedBy rdf:resource="http://www.digirati.com/ns/crowds#"/>
		<rdfs:range rdf:resource="xsd:boolean"/>
		<rdfs:comment>Boolean: defines whether an annotation body or set of annotation bodies should be used to generate an external resource, for example a topic page in a CMS system, which should be linked as the source of the annotation.</rdfs:comment>
		<rdfs:label>derivedAnnoExternalize</rdfs:label>
	</rdf:Property>
	<rdf:Property rdf:about="http://www.digirati.com/ns/crowds#derivedAnnoHumanReadable">
		<rdfs:isDefinedBy rdf:resource="http://www.digirati.com/ns/crowds#"/>
		<rdfs:range rdf:resource="xsd:boolean"/>
		<rdfs:comment>Boolean: defines whether an annotation body or set of annotation bodies should be converted to human readable plain text as a separate annotation body.</rdfs:comment>
		<rdfs:label>derivedAnnoHumanReadable</rdfs:label>
	</rdf:Property>
	<rdf:Property rdf:about="http://www.digirati.com/ns/crowds#derivedAnnoMotivatedBy">
		<rdfs:range rdf:resource="http://www.w3.org/ns/oa#Motivation"/>
		<rdfs:comment>The relationship between the derived Annotation produced from this user input, and a Motivation that describes the reason for the Annotation's creation.</rdfs:comment>
		<rdfs:isDefinedBy rdf:resource="http://www.digirati.com/ns/crowds#"/>
		<rdfs:label>derivedAnnoMotivatedBy</rdfs:label>
	</rdf:Property>
	<rdf:Property rdf:about="http://www.digirati.com/ns/crowds#derivedAnnoBodyPurpose">
		<rdfs:range rdf:resource="http://www.w3.org/ns/oa#Motivation"/>
		<rdfs:isDefinedBy rdf:resource="http://www.digirati.com/ns/crowds#"/>
		<rdfs:label>derivedAnnoBodyPurpose</rdfs:label>
		<rdfs:comment>The purpose served by the resource in the body of the derived Annotation.</rdfs:comment>
	</rdf:Property>
	<rdf:Property rdf:about="http://www.digirati.com/ns/crowds#derivedAnnoBodyFormat">
		<rdfs:range rdf:resource="http://purl.org/dc/terms/MediaTypeOrExtent"/>
		<rdfs:isDefinedBy rdf:resource="http://www.digirati.com/ns/crowds#"/>
		<rdfs:label>derivedAnnoBodyFormat</rdfs:label>
		<rdfs:comment>The format of the resource in the body of the derived Annotation (e.g. text/plain, application/html).</rdfs:comment>
	</rdf:Property>
	<rdf:Property rdf:about="http://www.digirati.com/ns/crowds#derivedAnnoBodyLabelParts">
		<rdfs:isDefinedBy rdf:resource="http://www.digirati.com/ns/crowds#"/>
		<rdfs:label>derivedAnnoBodyLabelParts</rdfs:label>
		<rdfs:comment>Field or fields in the model to concatenate to produce the label for the annotation body.</rdfs:comment>
	</rdf:Property>
	<rdf:Property rdf:about="http://www.digirati.com/ns/crowds#derivedAnnoBodyType">
		<rdfs:isDefinedBy rdf:resource="http://www.digirati.com/ns/crowds#"/>
		<rdfs:label>derivedAnnoBodyType</rdfs:label>
		<rdfs:comment>The type of the resource in the body of the derived Annotation (e.g. TextualBody, ExternalResource, etc.).</rdfs:comment>
	</rdf:Property>
</rdf:RDF>